fill out cp_to_ilp_new top

examples/pseudo_bool/cp_encoding/cp_to_ilp_newScript.sml
@@ -677,7 +677,7 @@ QED
 
 (*** abs ***)
 
-(* Only uses reifications *)
+(* abs only uses reifications *)
 
 (* Encoding for Y a variable *)
 Definition encode_abs_var_def:
@@ -744,282 +744,127 @@ Definition encode_abs_def:
   | INR cY => encode_abs_const X cY
 End
 
-(* TODO: not updated below here *)
-Theorem encode_abs_sem:
-  valid_assignment bnd wi
-  ⇒
-  EVERY (λx. iconstraint_sem x (wi,wb)) (encode_abs bnd X Y)
-  =
-  (
-  (case Y of INR _ => T | INL Y =>
-  (wb (Ge Y 0) ⇔ wi Y ≥ 0)) ∧
-  abs_sem X Y wi)
+Theorem encode_abs_sem_1:
+  valid_assignment bnd wi ∧
+  abs_sem X Y wi ⇒
+  EVERY (λx. iconstraint_sem x (wi,reify wi)) (encode_abs bnd X Y)
 Proof
   rw[encode_abs_def]>>
   TOP_CASE_TAC>>gvs[]
   >-
-    metis_tac[encode_abs_var_sem]
-  >>
-    metis_tac[encode_abs_const_sem]
+    simp[encode_abs_var_sem,reify_def,reify_reif_def]
+  >-
+    simp[encode_abs_const_sem,reify_def,reify_reif_def]
 QED
 
+Theorem encode_abs_sem_2:
+  valid_assignment bnd wi ∧
+  EVERY (λx. iconstraint_sem x (wi,wb)) (encode_abs bnd X Y) ⇒
+  abs_sem X Y wi
+Proof
+  rw[encode_abs_def]>>
+  every_case_tac>>gvs[]
+  >- rfs[encode_abs_var_sem]
+  >- rfs[encode_abs_const_sem]
+QED
 
-Definition encode_cp_one_def:
-  encode_cp_one bnd c =
-  case c of
-    NotEquals X Y => encode_not_equals bnd X Y
-  | AllDifferent As => encode_all_different bnd As
-  | Element R X As => encode_element bnd R X As
-  | Abs X Y => encode_abs bnd X Y
-  | Ilc Xs op rhs => encode_ilc Xs op rhs
+(*** ilc ***)
+
+(* ilc requires no extra variables *)
+Definition split_iclin_term_def:
+  (split_iclin_term ([]:'a iclin_term)
+    (acc:'a ilin_term) rhs = (acc,rhs)) ∧
+  (split_iclin_term ((c,X)::xs) acc rhs =
+    case X of
+      INL v => split_iclin_term xs ((c,v)::acc) rhs
+    | INR cc =>
+      split_iclin_term xs acc (rhs - c * cc))
 End
 
-Theorem encode_cp_one_sem_1:
-  valid_assignment bnd wi ∧
-  constraint_sem c wi ⇒
-  EVERY (λx. iconstraint_sem x (wi,reify_reif wi)) (encode_cp_one bnd c)
+Theorem split_iclin_term_sound:
+  ∀Xs rhs acc xs rhs'.
+    split_iclin_term Xs acc rhs = (xs,rhs') ⇒
+    eval_iclin_term wi Xs + eval_ilin_term wi acc - rhs =
+    eval_ilin_term wi xs - rhs'
 Proof
-  Cases_on`c`>>
-  rw[encode_cp_one_def,constraint_sem_def]
-  >- (
-    simp[encode_not_equals_sem,reify_reif_def]>>
-    gvs[not_equals_sem_def]>>
+  Induct
+  >-simp[split_iclin_term_def, eval_iclin_term_def, eval_ilin_term_def, iSUM_def]
+  >-(
+    Cases>>
+    Cases_on ‘r’>>
+    rw[split_iclin_term_def]>>
+    last_x_assum $ drule_then mp_tac>>
+    rw[eval_iclin_term_def, eval_ilin_term_def, iSUM_def, varc_def]>>
     intLib.ARITH_TAC)
-  >- (
-    simp[encode_all_different_sem,reify_reif_def]>>
-    gvs[all_different_sem_def,EL_ALL_DISTINCT_EL_EQ]>>
-    rw[]>>
-    first_x_assum(qspecl_then[`i`,`j`] mp_tac)>>
-    simp[EL_MAP]>>
+QED
+
+Theorem eval_lin_term_ge_1:
+  eval_lin_term wb (MAP (λe. (1, f e)) ls) ≥ 1 ⇔
+  ∃e. MEM e ls ∧ lit wb (f e)
+Proof
+  rw[eval_lin_term_def]>>
+  Induct_on ‘ls’>>
+  rw[iSUM_def,b2i_alt]
+  >-(
+    simp[SF DNF_ss]>>
+    qmatch_goalsub_abbrev_tac`_ + iSUM lss ≥ _`>>
+    `iSUM lss ≥ 0` by (
+      irule iSUM_ge_0>>
+      simp[Abbr`lss`,MEM_MAP,PULL_EXISTS,b2i_alt]>>
+      rw[])>>
     intLib.ARITH_TAC)
-  >- (
-    simp[encode_element_sem,reify_reif_def]>>
-    every_case_tac>>simp[])
-  >- (
-    simp[encode_abs_sem,reify_reif_def]>>
-    every_case_tac>>simp[])
-  >- (
-    simp[encode_ilc_sem,reify_reif_def]>>
-    every_case_tac>>simp[])
+  >- metis_tac[]
 QED
 
-Theorem encode_cp_one_sem_2:
-  valid_assignment bnd wi ∧
-  EVERY (λx. iconstraint_sem x (wi,wb)) (encode_cp_one bnd c) ⇒
-  constraint_sem c wi
-Proof
-  Cases_on`c`>>
-  rw[encode_cp_one_def,constraint_sem_def]
-  >-
-    gvs[encode_not_equals_sem]
-  >-
-    gvs[encode_all_different_sem]
-  >-
-    gvs[encode_element_sem]
-  >-
-    gvs[encode_abs_sem]
-  >-
-    gvs[encode_ilc_sem]
-QED
-
-(* An actual implementation will avoid duplicates here *)
-Definition encode_cp_all_def:
-  encode_cp_all bnd cs =
-  FLAT (MAP (encode_cp_one bnd) cs)
+Definition encode_ilc_def:
+  encode_ilc (Xs:'a iclin_term) (op:pbop) (rhs:int) =
+  let (xs,rhs) = split_iclin_term Xs [] rhs in
+  case op of
+    GreaterEqual => [(xs, [], rhs)]
+  | Greater => [(xs, [] , rhs+1)]
+  | LessEqual => [(MAP (λ(x:int, y). (-x, y)) xs, [], -rhs)]
+  | Less => [(MAP (λ(x:int, y). (-x, y)) xs, [], -rhs+1)]
+  | Equal => [(xs, [], rhs); (MAP (λ(x:int, y). (-x, y)) xs, [], -rhs)]
 End
 
-Theorem encode_cp_all_sem_1:
-  valid_assignment bnd wi ∧
-  EVERY (λc. constraint_sem c wi) cs ⇒
-  EVERY (λx. iconstraint_sem x (wi,reify_reif wi)) (encode_cp_all bnd cs)
+Theorem encode_ilc_sem:
+  EVERY (λx. iconstraint_sem x (wi,wb)) (encode_ilc Xs op rhs)
+  ⇔
+  ilc_sem Xs op rhs wi
 Proof
-  simp[encode_cp_all_def,EVERY_FLAT]>>
-  simp[Once EVERY_MEM]>>
-  rw[Once EVERY_MEM,MEM_MAP]>>
-  metis_tac[encode_cp_one_sem_1]
-QED
-
-Theorem encode_cp_all_sem_2:
-  valid_assignment bnd wi ∧
-  EVERY (λx. iconstraint_sem x (wi,wb)) (encode_cp_all bnd cs) ⇒
-  EVERY (λc. constraint_sem c wi) cs
-Proof
-  simp[encode_cp_all_def,EVERY_FLAT]>>
-  rw[Once EVERY_MEM,MEM_MAP,PULL_EXISTS]>>
-  simp[Once EVERY_MEM]>>
-  metis_tac[encode_cp_one_sem_2]
-QED
-
-(* === Examples ===
-
-not-equals
-  EVAL``encode_not_equals (λX. (-10,10)) (INL X) (INL Y)``
-  EVAL``encode_not_equals (λX. (-10,10)) (INL X) (INR 4)``
-
-all-different
-  EVAL``encode_all_different (λX. (-10,10)) [INL X; INL Y; INL Z; INR 0i]``
-
-element
-  EVAL``encode_element (λX. (-10,10)) (INL R) (INL X) [INL A; INL B; INL C; INL D; INL E]``
-
-abs
-  EVAL``encode_abs (λX. (-10,10)) (INL X) (INL Y)``
-
-*)
-
-
-
-Definition augment_assignment_def:
-  augment_assignment wb wc b =
-    case b of
-      INL b => wb b
-    | INR c => wc c
-End
-
-Definition augment_iassignment_def:
-  augment_iassignment (wi,wb) wc =
-  (wi, augment_assignment wb wc)
-End
-
-Definition exists_sem_def:
-  exists_sem (ls : ('a,('b + 'c)) iconstraint list)
-    (w :('a,'b) iassignment) ⇔
-  ∃wc: ('c -> bool).
-    EVERY (λc. iconstraint_sem c
-    (augment_iassignment w wc)) ls
-End
-
-Theorem encode_not_equals_sem:
-  valid_assignment bnd wi ⇒
-  (not_equals_sem X Y wi ⇔
-   exists_sem
-     (encode_not_equals bnd n X Y) (wi,wb))
-Proof
-  strip_tac>>
-  simp[exists_sem_def,not_equals_sem_def]>>
-  simp[encode_not_equals_def,bits_imply_sem,mk_constraint_ge_sem,augment_iassignment_def,augment_assignment_def]>>
-  eq_tac>>rw[]
-  >- (
-    qexists_tac`λb. varc wi X > varc wi Y`>>
-    simp[]>>
-    intLib.ARITH_TAC)>>
-  Cases_on`wc (Ne n X Y)`>>fs[]>>
+  rw[encode_ilc_def,ilc_sem_def]>>
+  pairarg_tac>>gvs[]>>
+  CASE_TAC>>
+  simp[iconstraint_sem_def, eval_lin_term_def, iSUM_def]>>
+  ‘∀xs. eval_ilin_term wi (MAP (λ(x,y). (-x,y)) xs) = -(eval_ilin_term wi xs)’ by (
+    Induct
+    >-simp[eval_ilin_term_def, iSUM_def]
+    >-(
+      Cases>>
+      pop_assum mp_tac>>
+      simp[eval_ilin_term_def, iSUM_def]>>
+      intLib.ARITH_TAC))>>
+  pop_assum (fn thm => simp[thm])>>
+  drule_then (qspec_then ‘wi’ mp_tac) split_iclin_term_sound>>
+  rw[Once eval_ilin_term_def, iSUM_def]>>
   intLib.ARITH_TAC
 QED
 
-(* Forgets a named variable *)
-Definition forget_var_def:
-  forget_var (ln,n:num) v =
-  case FLOOKUP ln v of
-    SOME m => (m, (ln,n))
-  | NONE =>
-    (n, (ln |+ (v,n),n+1))
-End
+(*** element ***)
 
-(* Forgets a literal name on the right *)
-Definition forget_lit_def:
-  forget_lit lnn l =
-  case l of
-    Pos (INR v) =>
-    let (n,lnn') = forget_var lnn v in
-      (Pos (INR n), lnn')
-  | Neg (INR v) =>
-    let (n,lnn') = forget_var lnn v in
-      (Neg (INR n), lnn')
-  | Pos (INL v) => (Pos (INL v), lnn)
-  | Neg (INL v) => (Neg (INL v), lnn)
-End
+(* element only uses reifications *)
 
-(* Forgets names in a lin term *)
-Definition forget_lin_term_def:
-  (forget_lin_term lnn [] =
-     ([],lnn)) ∧
-  (forget_lin_term lnn ((c,l)::ls) =
-    let (l',lnn') = forget_lit lnn l in
-    let (ls',lnn'') = forget_lin_term lnn' ls in
-    ((c,l')::ls', lnn''))
-End
-
-Definition forget_iconstraint_def:
-  forget_iconstraint lnn
-    ((is,bs,c) : ('a, 'a reif + 'a flag) iconstraint) =
-  let (bs',lnn') = forget_lin_term lnn bs in
-    ((is,bs',c),lnn')
-End
-
-(* Forget over an existentially quantified block *)
-Definition forget_exists_aux_def:
-  (forget_exists_aux lnn [] = ([],lnn)) ∧
-  (forget_exists_aux lnn (ic::ics) =
-    let (ic',lnn') = forget_iconstraint lnn ic in
-    let (ics',lnn'') = forget_exists_aux lnn' ics in
-    ((ic'::ics'),lnn''))
-End
-
-Definition forget_exists_def:
-  forget_exists n ics =
-    let (ics',lnn') = forget_exists_aux (FEMPTY,n) ics in
-    (ics',SND lnn')
-End
-
-Definition forget_all_aux_def:
-  (forget_all_aux n [] = []) ∧
-  (forget_all_aux n (ics::icss) =
-    let (ic',n') = forget_iconstraint lnn ic in
-      ic'::forget_all_aux
-    
-  [] = []) ∧
-  SND (FOLDL forget_exists (0n,[]) icss)
-End
-
-
-(* Forget the entire list of constraints *)
-Definition forget_all_def:
-  forget_all icss =
-  SND (FOLDL forget_exists (0n,[]) icss)
-End
-
-Definition exists_sem_def:
-  exists_sem (lss : ('a,('b + 'c)) iconstraint list list)
-    (w :('a,'b) iassignment) ⇔
-  EVERY
-    (λls.
-      ∃wc: ('c -> bool).
-        EVERY (λc. iconstraint_sem c
-          (augment_iassignment w wc)) ls) lss
-End
-
-
-
-Type iconstraint = ``:'a ilin_term # 'b lin_term # int``
-
-
-
-Definition fencode_not_equals_def:
-  fencode_not_equals bnd n X Y =
-  [
-    bits_imply bnd [Pos (Fresh n)] (mk_constraint_ge 1 X (-1) Y 1);
-    bits_imply bnd [Neg (Fresh n)] (mk_constraint_ge 1 Y (-1) X 1)
-  ]
-End
-
-Theorem foo:
-  forget (encode bnd n X Y)
-
-
-
-(* X_{=i} ⇒ Ai = R where Ai, R can be Varc *)
 Definition encode_element_eq_def:
   encode_element_eq bnd R X (i:num,Ai) =
   [
-    bits_imply bnd [Pos (Eq X (&(i+1)))] (mk_constraint_ge 1 Ai (-1) R 0);
-    bits_imply bnd [Pos (Eq X (&(i+1)))] (mk_constraint_ge 1 R (-1) Ai 0)
+    bits_imply bnd [Pos (INL (Eq X (&(i+1))))] (mk_constraint_ge 1 Ai (-1) R 0);
+    bits_imply bnd [Pos (INL (Eq X (&(i+1))))] (mk_constraint_ge 1 R (-1) Ai 0)
   ]
 End
 
 Theorem encode_element_eq_sem:
   valid_assignment bnd wi ∧
-  (wb (Eq X &(i+1)) ⇔ wi X = &(i+1))
+  (wb (INL (Eq X &(i+1))) ⇔ wi X = &(i+1))
   ⇒
   EVERY (λx. iconstraint_sem x (wi,wb)) (encode_element_eq bnd R X (i,Ai))
   =
@@ -1077,9 +922,9 @@ Theorem encode_element_var_sem:
   =
   (
   (∀i. 1 ≤ i ∧ i ≤ LENGTH As + 1 ⇒
-    (wb (Ge X &i) ⇔ wi X ≥ &i)) ∧
+    (wb (INL (Ge X &i)) ⇔ wi X ≥ &i)) ∧
   (∀i. 1 ≤ i ∧ i ≤ LENGTH As ⇒
-    (wb (Eq X &i) ⇔ wi X = &i)) ∧
+    (wb (INL (Eq X &i)) ⇔ wi X = &i)) ∧
   element_sem R (INL X) As wi)
 Proof
   rw[encode_element_var_def]>>
@@ -1180,528 +1025,98 @@ Definition encode_element_def:
   | INR cX => encode_element_const R cX As
 End
 
-(* TODO: This seem too precise *)
-Theorem encode_element_sem:
-  valid_assignment bnd wi
-  ⇒
-  EVERY (λx. iconstraint_sem x (wi,wb)) (encode_element bnd R X As)
-  =
-  (
-  (case X of INR _ => T | INL X =>
-  (∀i. 1 ≤ i ∧ i ≤ LENGTH As + 1 ⇒
-    (wb (Ge X &i) ⇔ wi X ≥ &i)) ∧
-  (∀i. 1 ≤ i ∧ i ≤ LENGTH As ⇒
-    (wb (Eq X &i) ⇔ wi X = &i))) ∧
-  element_sem R X As wi)
-Proof
-  rw[encode_element_def]>>
-  TOP_CASE_TAC>>gvs[]
-  >-
-    metis_tac[encode_element_var_sem]
-  >>
-    metis_tac[encode_element_const_sem]
-QED
-
-Definition reify_reif_def:
-  reify_reif wi eb ⇔
-  case eb of
-    Ge X i => wi X ≥ i
-  | Eq X i => wi X = i
-  | Ne X Y => varc wi X > varc wi Y
-  | Gem X Y => varc wi X ≥ varc wi Y
-  | Eqc X Y => varc wi X = varc wi Y
-End
-
 Theorem encode_element_sem_1:
   valid_assignment bnd wi ∧
   element_sem R X As wi ⇒
-  EVERY (λx. iconstraint_sem x (wi,reify_reif wi)) (encode_element bnd R X As)
+  EVERY (λx. iconstraint_sem x (wi,reify wi))
+    (encode_element bnd R X As)
 Proof
   rw[encode_element_def]>>
   TOP_CASE_TAC>>gvs[]
-  >- (
-    DEP_REWRITE_TAC [encode_element_var_sem]>>
-    simp[reify_reif_def])
-  >>
-    metis_tac[encode_element_const_sem]
+  >- simp[encode_element_var_sem,reify_def,reify_reif_def]
+  >- simp[encode_element_const_sem,reify_def,reify_reif_def]
 QED
 
 Theorem encode_element_sem_2:
   valid_assignment bnd wi ∧
-  EVERY (λx. iconstraint_sem x (wi,wb)) (encode_element bnd R X As) ⇒
+  EVERY (λx. iconstraint_sem x (wi,wb))
+    (encode_element bnd R X As) ⇒
   element_sem R X As wi
 Proof
   rw[encode_element_def]>>
   every_case_tac>>gvs[]
-  >- (
-    pop_assum mp_tac>>
-    DEP_REWRITE_TAC[encode_element_var_sem]>>
-    simp[])
-  >>
-    metis_tac[encode_element_const_sem]
+  >- rfs[encode_element_var_sem]
+  >- rfs[encode_element_const_sem]
 QED
 
-Theorem all_different_sem_aux:
-  (∀i j. i < j ∧ j < LENGTH As ⇒
-    let X = EL i As in
-    let Y = EL j As in
-    if wb (Ne X Y)
-    then varc wi X > varc wi Y
-    else varc wi Y > varc wi X) ⇒
-  all_different_sem As wi
-Proof
-  rw[all_different_sem_def,EL_ALL_DISTINCT_EL_EQ]>>
-  Cases_on`n1 = n2`>>simp[]>>
-  wlog_tac `n1 < n2` [`n1`,`n2`]
-  >- (
-    `n2 < n1` by fs[]>>
-    first_x_assum drule_all>>
-    simp[])>>
-  first_x_assum drule>>
-  rw[EL_MAP]>>
-  intLib.ARITH_TAC
-QED
-
-Theorem encode_all_different_sem:
-  valid_assignment bnd wi ⇒
-  EVERY (λx. iconstraint_sem x (wi,wb)) (encode_all_different bnd As)
-  =
-  (
-  (∀i j. i < j ∧ j < LENGTH As ⇒
-    let X = EL i As in
-    let Y = EL j As in
-    if wb (Ne X Y)
-    then varc wi X > varc wi Y
-    else varc wi Y > varc wi X) ∧
-  all_different_sem As wi)
-Proof
-  simp[MATCH_MP IMP_AND_LEFT all_different_sem_aux]>>
-  rw[encode_all_different_def, EVERY_FLAT, EVERY_GENLIST]>>
-  eq_tac>>rw[]>>
-  gvs[PULL_FORALL]
-  >- (
-    first_x_assum(qspecl_then[`i`,`j`] mp_tac)>>
-    simp[encode_not_equals_sem])>>
-  rw[]>>
-  first_x_assum drule_all>>
-  metis_tac[encode_not_equals_sem,not_equals_sem_aux]
-QED
-
-Definition split_iclin_term_def:
-  (split_iclin_term ([]:'a iclin_term)
-    (acc:'a ilin_term) rhs = (acc,rhs)) ∧
-  (split_iclin_term ((c,X)::xs) acc rhs =
-    case X of
-      INL v => split_iclin_term xs ((c,v)::acc) rhs
-    | INR cc =>
-      split_iclin_term xs acc (rhs - c * cc))
-End
-
-Theorem split_iclin_term_sound:
-  ∀Xs rhs acc xs rhs'.
-    split_iclin_term Xs acc rhs = (xs,rhs') ⇒
-    eval_iclin_term wi Xs + eval_ilin_term wi acc - rhs =
-    eval_ilin_term wi xs - rhs'
-Proof
-  Induct
-  >-simp[split_iclin_term_def, eval_iclin_term_def, eval_ilin_term_def, iSUM_def]
-  >-(
-    Cases>>
-    Cases_on ‘r’>>
-    rw[split_iclin_term_def]>>
-    last_x_assum $ drule_then mp_tac>>
-    rw[eval_iclin_term_def, eval_ilin_term_def, iSUM_def, varc_def]>>
-    intLib.ARITH_TAC)
-QED
-
-Definition encode_ilc_def:
-  encode_ilc (Xs:'a iclin_term) (op:pbop) (rhs:int) =
-  let (xs,rhs) = split_iclin_term Xs [] rhs in
-  case op of
-    GreaterEqual => [(xs, [], rhs)]
-  | Greater => [(xs, [] , rhs+1)]
-  | LessEqual => [(MAP (λ(x:int, y). (-x, y)) xs, [], -rhs)]
-  | Less => [(MAP (λ(x:int, y). (-x, y)) xs, [], -rhs+1)]
-  | Equal => [(xs, [], rhs); (MAP (λ(x:int, y). (-x, y)) xs, [], -rhs)]
-End
-
-Theorem encode_ilc_sem:
-  EVERY (λx. iconstraint_sem x (wi,wb)) (encode_ilc Xs op rhs)
-  ⇔
-  ilc_sem Xs op rhs wi
-Proof
-  rw[encode_ilc_def,ilc_sem_def]>>
-  pairarg_tac>>gvs[]>>
-  CASE_TAC>>
-  simp[iconstraint_sem_def, eval_lin_term_def, iSUM_def]>>
-  ‘∀xs. eval_ilin_term wi (MAP (λ(x,y). (-x,y)) xs) = -(eval_ilin_term wi xs)’ by (
-    Induct
-    >-simp[eval_ilin_term_def, iSUM_def]
-    >-(
-      Cases>>
-      pop_assum mp_tac>>
-      simp[eval_ilin_term_def, iSUM_def]>>
-      intLib.ARITH_TAC))>>
-  pop_assum (fn thm => simp[thm])>>
-  drule_then (qspec_then ‘wi’ mp_tac) split_iclin_term_sound>>
-  rw[Once eval_ilin_term_def, iSUM_def]>>
-  intLib.ARITH_TAC
-QED
-
-Theorem eval_lin_term_ge_1:
-  eval_lin_term wb (MAP (λe. (1, f e)) ls) ≥ 1 ⇔
-  ∃e. MEM e ls ∧ lit wb (f e)
-Proof
-  rw[eval_lin_term_def]>>
-  Induct_on ‘ls’>>
-  rw[iSUM_def,b2i_alt]
-  >-(
-    simp[SF DNF_ss]>>
-    qmatch_goalsub_abbrev_tac`_ + iSUM lss ≥ _`>>
-    `iSUM lss ≥ 0` by (
-      irule iSUM_ge_0>>
-      simp[Abbr`lss`,MEM_MAP,PULL_EXISTS,b2i_alt]>>
-      rw[])>>
-    intLib.ARITH_TAC)
-  >- metis_tac[]
-QED
-
-(* Encodes that all As ≥ M *)
-Definition encode_Gem_ge_def:
-  encode_Gem_ge bnd As M =
-  MAP (λA. bits_imply bnd [Pos (Gem A M)] (mk_constraint_ge 1 A (-1) M 0)) As
-End
-
-(* iff versions *)
-Definition encode_Gem_ge_iff_def:
-  encode_Gem_ge_iff bnd As M =
-  encode_Gem_ge bnd As M ++
-  MAP (λA. bits_imply bnd [Neg (Gem A M)] (mk_constraint_ge 1 M (-1) A 1)) As
-End
-
-(* Encodes that all As ≤ M *)
-Definition encode_Gem_le_def:
-  encode_Gem_le bnd As M =
-  MAP (λA. bits_imply bnd [Pos (Gem M A)] (mk_constraint_ge 1 M (-1) A 0)) As
-End
-
-Definition encode_Gem_le_iff_def:
-  encode_Gem_le_iff bnd As M =
-  encode_Gem_le bnd As M ++
-  MAP (λA. bits_imply bnd [Neg (Gem M A)] (mk_constraint_ge 1 A (-1) M 1)) As
-End
-
-Theorem encode_Gem_ge_sem:
-  valid_assignment bnd wi ⇒
-  EVERY (λx. iconstraint_sem x (wi,wb)) (encode_Gem_ge bnd As M) =
-    (∀A. MEM A As ∧ wb (Gem A M) ⇒ varc wi A ≥ varc wi M)
-Proof
-  rw[encode_Gem_ge_def]>>
-  simp[EVERY_MAP,EVERY_MEM,bits_imply_sem,mk_constraint_ge_sem,GSYM integerTheory.INT_POLY_CONV_rth,integerTheory.INT_GE, integerTheory.INT_SUB_LE]>>
-  metis_tac[]
-QED
-
-Theorem encode_Gem_le_sem:
-  valid_assignment bnd wi ⇒
-  EVERY (λx. iconstraint_sem x (wi,wb)) (encode_Gem_le bnd As M) =
-    (∀A. MEM A As ∧ wb (Gem M A) ⇒ varc wi A ≤ varc wi M)
-Proof
-  rw[encode_Gem_le_def]>>
-  simp[EVERY_MAP,EVERY_MEM,bits_imply_sem,mk_constraint_ge_sem,GSYM integerTheory.INT_POLY_CONV_rth,integerTheory.INT_GE, integerTheory.INT_SUB_LE]>>
-  metis_tac[]
-QED
-
-Theorem encode_Gem_ge_iff_sem:
-  valid_assignment bnd wi ⇒
-  EVERY (λx. iconstraint_sem x (wi,wb)) (encode_Gem_ge_iff bnd As M) =
-    (∀A. MEM A As ⇒ (wb (Gem A M) ⇔ varc wi A ≥ varc wi M))
-Proof
-  rw[encode_Gem_ge_iff_def,encode_Gem_ge_sem]>>
-  simp[EVERY_MAP,EVERY_MEM,bits_imply_sem,mk_constraint_ge_sem,
-    intLib.ARITH_PROVE ``X + -1 * (Y:int) ≥ 1 ⇔ ¬ (Y ≥ X)``]>>
-  metis_tac[]
-QED
-
-Theorem encode_Gem_le_iff_sem:
-  valid_assignment bnd wi ⇒
-  EVERY (λx. iconstraint_sem x (wi,wb)) (encode_Gem_le_iff bnd As M) =
-    (∀A. MEM A As ⇒ (wb (Gem M A) ⇔ varc wi A ≤ varc wi M))
-Proof
-  rw[encode_Gem_le_iff_def,encode_Gem_le_sem]>>
-  simp[EVERY_MAP,EVERY_MEM,bits_imply_sem,mk_constraint_ge_sem,
-    intLib.ARITH_PROVE ``X + -1 * (Y:int) ≥ 1 ⇔ ¬ (X <= Y)``]>>
-  metis_tac[]
-QED
-
-Definition encode_arr_max_def:
-  encode_arr_max bnd M As =
-  ([], MAP (λA. (1, Pos (Gem A M))) As, 1) ::
-  encode_Gem_ge bnd As M ++
-  MAP (λA. mk_constraint_ge 1 M (-1) A 0) As
-End
-
-Theorem encode_arr_max_sem:
-  valid_assignment bnd wi ⇒
-  EVERY (λx. iconstraint_sem x (wi,wb)) (encode_arr_max bnd M As) = (
-    (∃A. MEM A As ∧ wb (Gem A M)) ∧
-    (∀A. MEM A As ∧ wb (Gem A M) ⇒ varc wi A ≥ varc wi M) ∧
-    arr_max_sem M As wi)
-Proof
-  strip_tac>>
-  simp[encode_arr_max_def,encode_Gem_ge_sem]>>
-  match_mp_tac LEFT_AND_CONG>>
-  CONJ_TAC >-
-    simp[iconstraint_sem_def,eval_ilin_term_def,iSUM_def,eval_lin_term_ge_1]>>
-  strip_tac>>
-  match_mp_tac LEFT_AND_CONG>> simp[]>>
-  strip_tac>>
-  simp[arr_max_sem_def,EVERY_MAP,mk_constraint_ge_sem,GSYM integerTheory.INT_POLY_CONV_rth,
-       integerTheory.INT_GE,integerTheory.INT_SUB_LE,MEM_MAP,EVERY_MEM]>>
-  iff_tac>>
-  rw[]>>
-  pop_assum drule>>
-  pop_assum drule>>
-  rw[integerTheory.INT_GE,GSYM integerTheory.INT_LE_ANTISYM]>>
-  simp[SF SFY_ss]
-QED
-
-Definition encode_arr_min_def:
-  encode_arr_min bnd M As =
-  ([], MAP (λA. (1, Pos (Gem M A))) As, 1) ::
-  encode_Gem_le bnd As M ++
-  MAP (λA. mk_constraint_ge 1 A (-1) M 0) As
-End
-
-Theorem encode_arr_min_sem:
-  valid_assignment bnd wi ⇒
-  EVERY (λx. iconstraint_sem x (wi,wb)) (encode_arr_min bnd M As) = (
-    (∃A. MEM A As ∧ wb (Gem M A)) ∧
-    (∀A. MEM A As ∧ wb (Gem M A) ⇒ varc wi A ≤ varc wi M) ∧
-    arr_min_sem M As wi)
-Proof
-  strip_tac>>
-  simp[encode_arr_min_def,encode_Gem_le_sem]>>
-  match_mp_tac LEFT_AND_CONG>>
-  CONJ_TAC >-
-    simp[iconstraint_sem_def,eval_ilin_term_def,iSUM_def,eval_lin_term_ge_1]>>
-  strip_tac>>
-  match_mp_tac LEFT_AND_CONG>> simp[]>>
-  strip_tac>>
-  simp[arr_min_sem_def,EVERY_MAP,mk_constraint_ge_sem,GSYM integerTheory.INT_POLY_CONV_rth,
-       integerTheory.INT_GE,integerTheory.INT_SUB_LE,MEM_MAP,EVERY_MEM]>>
-  iff_tac>>
-  rw[]>>
-  pop_assum drule>>
-  pop_assum drule>>
-  rw[integerTheory.INT_GE,GSYM integerTheory.INT_LE_ANTISYM]>>
-  simp[SF SFY_ss]
-QED
-
-Definition encode_count_def:
-  encode_count bnd Y C As =
-  let
-    ilpc =
-    case C of
-      INL vC => [
-        ([(-1, vC)], MAP (λA. (1, Pos (Eqc A Y))) As, 0);
-        ([(1, vC)], MAP (λA. (-1, Pos (Eqc A Y))) As, 0)]
-    | INR cC => [
-        ([], MAP (λA. (1, Pos (Eqc A Y))) As, cC);
-        ([], MAP (λA. (-1, Pos (Eqc A Y))) As, -cC)]
-  in
-    encode_Gem_ge_iff bnd As Y ++
-    encode_Gem_le_iff bnd As Y ++
-    MAP (λA. bits_imply bnd [Pos (Eqc A Y)]
-                        ([], [(1, Pos (Gem A Y)); (1, Pos (Gem Y A))], 2)) As ++
-    MAP (λA. bits_imply bnd [Neg (Eqc A Y)]
-                        ([], [(1, Neg (Gem A Y)); (1, Neg (Gem Y A))], 1)) As ++
-    ilpc
-End
-
-Theorem iSUM_MAP_lin:
-  ∀ls a f b. iSUM (MAP (λx. a * f x + b) ls) = a * iSUM (MAP (λx. f x) ls) + b * &LENGTH ls
-Proof
-  Induct>>
-  simp[iSUM_def,MAP,LENGTH]>>
-  rw[]>>
-  intLib.ARITH_TAC
-QED
-
-Theorem iSUM_MAP_lin_const = iSUM_MAP_lin |> CONV_RULE (RESORT_FORALL_CONV List.rev) |> Q.SPEC `0` |> SRULE [] |> SPEC_ALL;
-
-Theorem b2i_ge_2[simp]:
-  b2i b1 + b2i b2 ≥ 2 ⇔ b1 ∧ b2
-Proof
-  rw[b2i_alt]
-QED
-
-Theorem b2i_ge_1[simp]:
-  b2i b1 + b2i b2 ≥ 1 ⇔ b1 ∨ b2
-Proof
-  rw[b2i_alt]
-QED
-
-Theorem encode_count_sem:
-  valid_assignment bnd wi ⇒
-  EVERY (λx. iconstraint_sem x (wi,wb)) (encode_count bnd Y C As) = (
-    EVERY (λA. wb (Gem A Y) ⇔ varc wi A ≥ varc wi Y) As ∧
-    EVERY (λA. wb (Gem Y A) ⇔ varc wi Y ≥ varc wi A) As ∧
-    EVERY (λA. wb (Eqc A Y) ⇔ varc wi A = varc wi Y) As ∧
-    count_sem Y C As wi)
-Proof
-  strip_tac>>
-  simp[encode_count_def]>>
-  simp[GSYM CONJ_ASSOC]>>
-  ho_match_mp_tac LEFT_AND_CONG>>
-  CONJ_TAC >-
-    simp[encode_Gem_ge_iff_sem,EVERY_MEM]>>
-  strip_tac>>
-  ho_match_mp_tac LEFT_AND_CONG>>
-  CONJ_TAC >-
-    simp[encode_Gem_le_iff_sem,EVERY_MEM,integerTheory.INT_GE]>>
-  strip_tac>>
-  simp[CONJ_ASSOC]>>
-  ho_match_mp_tac LEFT_AND_CONG>>
-  CONJ_TAC >- (
-    fs[EVERY_MEM,MEM_MAP,PULL_EXISTS,bits_imply_sem,iconstraint_sem_def,eval_ilin_term_def,eval_lin_term_def,iSUM_def]>>
-    metis_tac[integerTheory.INT_LE_ANTISYM,integerTheory.INT_GE])>>
-  strip_tac
-  >- (
-    Cases_on ‘C’>>
-    simp[count_sem_def]>>
-    rw[METIS_PROVE[] “∀P a b. (∀x. x = a ∨ x = b ⇒ P x) ⇔ P a ∧ P b”]>>
-    simp[iconstraint_sem_def,eval_ilin_term_def,eval_lin_term_def,
-      MAP_MAP_o,combinTheory.o_ABS_R,b2i_alt,iSUM_def,Once varc_def]>>
-    ‘iSUM (MAP (λA. if wb (Eqc A Y) then 1 else 0) As) =
-     iSUM (MAP (λA. if varc wi A = varc wi Y then 1 else 0) As)’ by
-      fs[EVERY_MEM,Cong MAP_CONG]>>
-    simp[iSUM_MAP_lin_const]>>
-    intLib.ARITH_TAC)
-QED
-
-(* domain of X given by bnd *)
-Definition dom_def:
-  dom bnd X =
-  case X of
-    INL vX =>
-      let
-        (lb, ub) = bnd vX
-      in
-        if lb > ub then [] else GENLIST (λn. &n + lb) (Num (ub - lb) + 1)
-  | INR cX => [cX]
-End
-
-Definition encode_nvalue_def:
-  encode_nvalue bnd Y As =
-  let
-    Vals = nub $ FLAT $ MAP (dom bnd) As;
-    some_eq = λv. ([], MAP (λA. (1i, Pos (Eqc A (INR v)))) As, 1i);
-    none_eq = λv. ([], MAP (λA. (-1i, Pos (Eqc A (INR v)))) As, 0i)
-  in
-    MAP (λv. bits_imply bnd [Pos (Nv As v)] (some_eq v)) Vals ++
-    MAP (λv. bits_imply bnd [Neg (Nv As v)] (none_eq v)) Vals ++
-    (case Y of
-        INL vY =>
-          [([(-1, vY)], MAP (λv. (1i, Pos (Nv As v))) Vals, 0);
-          ([(1, vY)], MAP (λv. (-1i, Pos (Nv As v))) Vals, 0)]
-      | INR cY =>
-          [([], MAP (λv. (1i, Pos (Nv As v))) Vals, cY);
-          ([], MAP (λv. (-1i, Pos (Nv As v))) Vals, -cY)])
-End
-
-(* TODO: Theorem encode_nvalue_sem *)
-
-Definition encode_table_def:
-  encode_table bnd Xs Tss =
-  let n = LENGTH Xs in
-    if EVERY (λTs. LENGTH Ts = n) Tss
-    then
-      let
-        all_eq = λTs. ([], MAP (λ(X, T). (1i, Pos (Eqc X T))) (ZIP (Xs, Ts)), &n);
-        some_neq = λTs. ([], MAP (λ(X, T). (-1i, Pos (Eqc X T))) (ZIP (Xs, Ts)), -&n + 1i)
-      in
-        MAP (λTs. bits_imply bnd [Pos (Tb Xs Ts &n)] (all_eq Ts)) Tss ++
-        MAP (λTs. bits_imply bnd [Neg (Tb Xs Ts &n)] (some_neq Ts)) Tss ++
-        [([], MAP (λTs. (1i, Pos (Tb Xs Ts &n))) Tss, 1i)]
-    else [([], [], 1i)]
-End
-
-(* TODO: Theorem encode_table_sem *)
-
-(* The top-level encodings *)
+(* TODO below *)
 Definition encode_cp_one_def:
-  encode_cp_one bnd c =
+  encode_cp_one bnd n c =
   case c of
-    NotEquals X Y => encode_not_equals bnd X Y
-  | AllDifferent As => encode_all_different bnd As
-  | Element R X As => encode_element bnd R X As
-  | Abs X Y => encode_abs bnd X Y
-  | Ilc Xs op rhs => encode_ilc Xs op rhs
+    NotEquals X Y => encode_not_equals bnd n X Y
+  | AllDifferent As => encode_all_different bnd n As
+  | Element R X As => (n, encode_element bnd R X As)
+  | Abs X Y => (n, encode_abs bnd X Y)
+  | Ilc Xs op rhs => (n, encode_ilc Xs op rhs)
 End
+
+Definition cencode_cp_one_def:
+  cencode_cp_one bnd n c =
+  (I ## forget_b_ilps) (encode_cp_one bnd n c)
+End
+
+(* TODO: push the ## inside *)
+Theorem cencode_cp_one_compute =
+  SRULE [encode_cp_one_def] cencode_cp_one_def;
 
 Theorem encode_cp_one_sem_1:
   valid_assignment bnd wi ∧
   constraint_sem c wi ⇒
-  EVERY (λx. iconstraint_sem x (wi,reify_reif wi)) (encode_cp_one bnd c)
+  EVERY (λx. iconstraint_sem x (wi,reify wi)) (SND (encode_cp_one bnd n c))
 Proof
   Cases_on`c`>>
   rw[encode_cp_one_def,constraint_sem_def]
-  >- (
-    simp[encode_not_equals_sem,reify_reif_def]>>
-    gvs[not_equals_sem_def]>>
-    intLib.ARITH_TAC)
-  >- (
-    simp[encode_all_different_sem,reify_reif_def]>>
-    gvs[all_different_sem_def,EL_ALL_DISTINCT_EL_EQ]>>
-    rw[]>>
-    first_x_assum(qspecl_then[`i`,`j`] mp_tac)>>
-    simp[EL_MAP]>>
-    intLib.ARITH_TAC)
-  >- (
-    simp[encode_element_sem,reify_reif_def]>>
-    every_case_tac>>simp[])
-  >- (
-    simp[encode_abs_sem,reify_reif_def]>>
-    every_case_tac>>simp[])
-  >- (
-    simp[encode_ilc_sem,reify_reif_def]>>
-    every_case_tac>>simp[])
+  >- metis_tac[encode_not_equals_sem_1]
+  >- metis_tac[encode_all_different_sem_1]
+  >- metis_tac[encode_element_sem_1]
+  >- cheat
+  >- metis_tac[encode_abs_sem_1]
+  >- metis_tac[encode_ilc_sem]
+  >> cheat
 QED
 
 Theorem encode_cp_one_sem_2:
   valid_assignment bnd wi ∧
-  EVERY (λx. iconstraint_sem x (wi,wb)) (encode_cp_one bnd c) ⇒
+  EVERY (λx. iconstraint_sem x (wi,wb)) (SND (encode_cp_one bnd n c)) ⇒
   constraint_sem c wi
 Proof
   Cases_on`c`>>
   rw[encode_cp_one_def,constraint_sem_def]
-  >-
-    gvs[encode_not_equals_sem]
-  >-
-    gvs[encode_all_different_sem]
-  >-
-    gvs[encode_element_sem]
-  >-
-    gvs[encode_abs_sem]
-  >-
-    gvs[encode_ilc_sem]
+  >- metis_tac[encode_not_equals_sem_2]
+  >- metis_tac[encode_all_different_sem_2]
+  >- metis_tac[encode_element_sem_2]
+  >- cheat
+  >- metis_tac[encode_abs_sem_2]
+  >- metis_tac[encode_ilc_sem]
+  >> cheat
 QED
 
-(* An actual implementation will avoid duplicates here *)
-Definition encode_cp_all_def:
-  encode_cp_all bnd cs =
-  FLAT (MAP (encode_cp_one bnd) cs)
+(* An actual implementation will avoid duplicates here,
+  probably with an accumulator *)
+Definition cencode_cp_all_def:
+  (cencode_cp_all bnd n [] = []) ∧
+  (cencode_cp_all bnd n (c::cs) =
+    let (n',c') = cencode_cp_one bnd n c in
+    c' ++ cencode_cp_all bnd n' cs)
 End
 
 Theorem encode_cp_all_sem_1:
   valid_assignment bnd wi ∧
   EVERY (λc. constraint_sem c wi) cs ⇒
-  EVERY (λx. iconstraint_sem x (wi,reify_reif wi)) (encode_cp_all bnd cs)
+  ∃wb.
+  EVERY (λx. iconstraint_sem x (wi,wb)) (cencode_cp_all bnd n cs)
 Proof
-  simp[encode_cp_all_def,EVERY_FLAT]>>
-  simp[Once EVERY_MEM]>>
-  rw[Once EVERY_MEM,MEM_MAP]>>
-  metis_tac[encode_cp_one_sem_1]
+  cheat
 QED
 
 Theorem encode_cp_all_sem_2:
@@ -1709,20 +1124,17 @@ Theorem encode_cp_all_sem_2:
   EVERY (λx. iconstraint_sem x (wi,wb)) (encode_cp_all bnd cs) ⇒
   EVERY (λc. constraint_sem c wi) cs
 Proof
-  simp[encode_cp_all_def,EVERY_FLAT]>>
-  rw[Once EVERY_MEM,MEM_MAP,PULL_EXISTS]>>
-  simp[Once EVERY_MEM]>>
-  metis_tac[encode_cp_one_sem_2]
+  cheat
 QED
 
 (* === Examples ===
 
 not-equals
-  EVAL``encode_not_equals (λX. (-10,10)) (INL X) (INL Y)``
-  EVAL``encode_not_equals (λX. (-10,10)) (INL X) (INR 4)``
+  EVAL``encode_not_equals (λX. (-10,10)) 5 (INL X) (INL Y)``
+  EVAL``encode_not_equals (λX. (-10,10)) 5 (INL X) (INR 4)``
 
 all-different
-  EVAL``encode_all_different (λX. (-10,10)) [INL X; INL Y; INL Z; INR 0i]``
+  EVAL``encode_all_different (λX. (-10,10)) 5 [INL X; INL Y; INL Z; INR 0i]``
 
 element
   EVAL``encode_element (λX. (-10,10)) (INL R) (INL X) [INL A; INL B; INL C; INL D; INL E]``
